Fixed some extra theories (pred_set,real) for tight equalities

examples/diningcryptos/extra_realScript.sml
@@ -1,33 +1,10 @@
-(* interactive mode
-loadPath := ["../ho_prover","../subtypes","../rsa"] @ !loadPath;
-app load ["bossLib","realLib","transcTheory","subtypeTheory",
-          "hurdUtils","extra_boolTheory",
-          "boolContext","extra_pred_setTools","sumTheory"];
+open HolKernel Parse boolLib bossLib;
 
-open HolKernel Parse boolLib bossLib realTheory realLib
-     hurdUtils subtypeTheory extra_numTheory transcTheory
-     pred_setTheory arithmeticTheory seqTheory combinTheory pairTheory
-     extra_pred_setTheory extra_boolTheory extra_pred_setTools
-     sumTheory;
-
-
-loadPath := ["../subtypes"] @ !loadPath;
-app load ["bossLib","realLib","transcTheory","subtypeTheory",
-          "hurdUtils","extra_boolTheory",
-          "extra_pred_setTheory","sumTheory"];
-
-quietdec := true;
-*)
-
-open HolKernel Parse boolLib bossLib realTheory realLib
+open realTheory realLib util_probTheory
      hurdUtils subtypeTheory extra_numTheory transcTheory
      pred_setTheory arithmeticTheory seqTheory combinTheory pairTheory
      extra_pred_setTheory extra_boolTheory real_sigmaTheory
      sumTheory limTheory listTheory rich_listTheory;
-
-(* interactive mode
-quietdec := false;
-*)
 
 val _ = new_theory "extra_real";
 
@@ -35,38 +12,30 @@ val _ = new_theory "extra_real";
 (* Tools.                                                                    *)
 (* ------------------------------------------------------------------------- *)
 
-val Reverse = Tactical.REVERSE;
-val REVERSE = Tactical.REVERSE;
-val Strip = rpt (POP_ASSUM MP_TAC) >> rpt STRIP_TAC;
 val Simplify = RW_TAC arith_ss;
-val Suff = PARSE_TAC SUFF_TAC;
-val Know = PARSE_TAC KNOW_TAC;
-val Rewr = DISCH_THEN (REWRITE_TAC o wrap);
-val Rewr' = DISCH_THEN (ONCE_REWRITE_TAC o wrap);
-val STRONG_DISJ_TAC = CONV_TAC (REWR_CONV (GSYM IMP_DISJ_THM)) >> STRIP_TAC;
-val Cond =
-  DISCH_THEN
-  (fn mp_th =>
-   let
-     val cond = fst (dest_imp (concl mp_th))
-   in
-     KNOW_TAC cond >| [ALL_TAC, DISCH_THEN (MP_TAC o MP mp_th)]
-   end);
-
-val POP_ORW = POP_ASSUM (fn thm => ONCE_REWRITE_TAC [thm]);
 
 (* ------------------------------------------------------------------------- *)
 (* Definitions.                                                              *)
 (* ------------------------------------------------------------------------- *)
 
-val inf_def = Define `inf p = ~(sup (IMAGE $~ p))`;
+Theorem inf_alt : (* was: inf_def *)
+    !p. inf p = ~(sup (IMAGE $~ p))
+Proof
+    RW_TAC real_ss [inf_def]
+ >> Suff `(\r. p (-r)) = (IMAGE numeric_negate p)` >- rw []
+ >> SET_EQ_TAC
+ >> RW_TAC std_ss [IN_IMAGE, IN_APP]
+ >> EQ_TAC >> RW_TAC std_ss []
+ >- (Q.EXISTS_TAC `-x` >> rw [REAL_NEG_NEG])
+ >> rw [REAL_NEG_NEG]
+QED
 
 val zreal_def = Define `zreal (x : real) = (x = 0)`;
 val nzreal_def = Define `nzreal (x : real) = ~(x = 0)`;
-val posreal_def = Define `posreal (x : real) = 0 < x`;
-val nnegreal_def = Define `nnegreal (x : real) = 0 <= x`;
-val negreal_def = Define `negreal (x : real) = 0 < ~x`;
-val nposreal_def = Define `nposreal (x : real) = 0 <= ~x`;
+val posreal_def = Define `posreal (x : real) = (0 < x)`;
+val nnegreal_def = Define `nnegreal (x : real) = (0 <= x)`;
+val negreal_def = Define `negreal (x : real) = (0 < ~x)`;
+val nposreal_def = Define `nposreal (x : real) = (0 <= ~x)`;
 
 (* ------------------------------------------------------------------------- *)
 (* Theorems.                                                                 *)
@@ -76,7 +45,7 @@ val INF_DEF_ALT = store_thm
   ("INF_DEF_ALT",
    ``!p. inf p = ~(sup (\r. ~r IN p))``,
    RW_TAC std_ss []
-   >> PURE_REWRITE_TAC [inf_def, IMAGE_DEF]
+   >> PURE_REWRITE_TAC [inf_alt, IMAGE_DEF]
    >> Suff `{~x | x IN p} = (\r:real. ~r IN p)`
    >- RW_TAC std_ss []
    >> RW_TAC std_ss [EXTENSION]
@@ -88,138 +57,11 @@ val REAL_LE_EQ = store_thm
    ``!(x:real) y. x <= y /\ y <= x ==> (x = y)``,
    REAL_ARITH_TAC);
 
-val REAL_SUP_EXISTS_UNIQUE = store_thm
-  ("REAL_SUP_EXISTS_UNIQUE",
-   ``!P. (?(x:real). P x) /\ (?z. !x. P x ==> x <= z)
-         ==> (?!s. !y. (?x. P x /\ y < x) = y < s)``,
-   REPEAT STRIP_TAC
-   >> CONV_TAC EXISTS_UNIQUE_CONV
-   >> RW_TAC std_ss [] >|
-   [ASSUME_TAC (SPEC ``P:real->bool`` REAL_SUP_LE)
-    >> PROVE_TAC [],
-    Suff `~((s:real) < s') /\ ~(s' < s)`
-      >- (KILL_TAC >> REAL_ARITH_TAC)
-    >> REPEAT STRIP_TAC >|
-    [Suff `!(x:real). P x ==> ~(s < x)` >- PROVE_TAC []
-     >> REPEAT STRIP_TAC
-     >> Suff `~((s:real) < s)` >- PROVE_TAC []
-     >> KILL_TAC
-     >> REAL_ARITH_TAC,
-     Suff `!(x:real). P x ==> ~(s' < x)` >- PROVE_TAC []
-     >> REPEAT STRIP_TAC
-     >> Suff `~((s':real) < s')` >- PROVE_TAC []
-     >> KILL_TAC
-     >> REAL_ARITH_TAC]]);
-
-val REAL_SUP_MAX = store_thm
-  ("REAL_SUP_MAX",
-   ``!P z. P z /\ (!x. P x ==> x <= z) ==> (sup P = z)``,
-    REPEAT STRIP_TAC
-    >> Know `!(y:real). (?x. P x /\ y < x) = y < z`
-    >- (STRIP_TAC
-        >> EQ_TAC >|
-        [REPEAT STRIP_TAC
-         >> PROVE_TAC [REAL_ARITH ``(y:real) < x /\ x <= z ==> y < z``],
-         PROVE_TAC []])
-    >> STRIP_TAC
-    >> Know `!y. (?x. P x /\ y < x) = y < sup P`
-    >- PROVE_TAC [REAL_SUP_LE]
-    >> STRIP_TAC
-    >> Know `(?(x:real). P x) /\ (?z. !x. P x ==> x <= z)`
-    >- PROVE_TAC []
-    >> STRIP_TAC
-    >> ASSUME_TAC ((SPEC ``P:real->bool`` o CONV_RULE
-                      (DEPTH_CONV EXISTS_UNIQUE_CONV)) REAL_SUP_EXISTS_UNIQUE)
-    >> RES_TAC);
-
-val REAL_INF_MIN = store_thm
-  ("REAL_INF_MIN",
-   ``!p z. z IN p /\ (!x. x IN p ==> z <= x) ==> (inf p = z)``,
-   RW_TAC std_ss [SPECIFICATION]
-   >> MP_TAC (SPECL [``(\r. (p:real->bool) (~r))``, ``~(z:real)``]
-              REAL_SUP_MAX)
-   >> RW_TAC std_ss [REAL_NEGNEG, INF_DEF_ALT, SPECIFICATION]
-   >> Suff `!x. p ~x ==> x <= ~z`
-   >- PROVE_TAC [REAL_ARITH ``~~(x:real) = x``]
-   >> REPEAT STRIP_TAC
-   >> Suff `z <= ~x` >- (KILL_TAC >> REAL_ARITH_TAC)
-   >> PROVE_TAC []);
-
-val HALF_POS = store_thm
-  ("HALF_POS",
-   ``0 < 1/2``,
-   PROVE_TAC [REAL_ARITH ``0:real < 1``, REAL_LT_HALF1]);
-
-val HALF_CANCEL = store_thm
-  ("HALF_CANCEL",
-   ``2 * (1 / 2) = 1``,
-   Suff `2 * inv 2 = 1` >- PROVE_TAC [REAL_INV_1OVER]
-   >> PROVE_TAC [REAL_MUL_RINV, REAL_ARITH ``~(2:real = 0)``]);
-
-val POW_HALF_POS = store_thm
-  ("POW_HALF_POS",
-   ``!n. 0 < (1/2) pow n``,
-   STRIP_TAC
-   >> Cases_on `n` >- PROVE_TAC [REAL_ARITH ``0:real < 1``, pow]
-   >> PROVE_TAC [HALF_POS, POW_POS_LT]);
-
-val POW_HALF_MONO = store_thm
-  ("POW_HALF_MONO",
-   ``!m n. m <= n ==> (1/2) pow n <= (1/2) pow m``,
-   REPEAT STRIP_TAC
-   >> Induct_on `n` >|
-   [STRIP_TAC
-    >> Know `m:num = 0` >- DECIDE_TAC
-    >> PROVE_TAC [REAL_ARITH ``a:real <= a``],
-    Cases_on `m = SUC n` >- PROVE_TAC [REAL_ARITH ``a:real <= a``]
-    >> ONCE_REWRITE_TAC [pow]
-    >> STRIP_TAC
-    >> Know `m:num <= n` >- DECIDE_TAC
-    >> STRIP_TAC
-    >> Suff `2 * ((1/2) * (1/2) pow n) <= 2 * (1/2) pow m`
-    >- PROVE_TAC [REAL_ARITH ``0:real < 2``, REAL_LE_LMUL]
-    >> Suff `(1/2) pow n <= 2 * (1/2) pow m`
-    >- (KILL_TAC
-        >> PROVE_TAC [GSYM REAL_MUL_ASSOC, HALF_CANCEL, REAL_MUL_LID])
-    >> PROVE_TAC [REAL_ARITH ``!x y. 0:real < x /\ x <= y ==> x <= 2 * y``,
-                  POW_HALF_POS]]);
-
 val POW_HALF_TWICE = store_thm
   ("POW_HALF_TWICE",
    ``!n. (1 / 2) pow n = 2 * (1 / 2) pow (SUC n)``,
    RW_TAC std_ss [pow, REAL_MUL_ASSOC]
    >> PROVE_TAC [HALF_CANCEL, REAL_MUL_LID]);
-
-val X_HALF_HALF = store_thm
-  ("X_HALF_HALF",
-   ``!x. 1/2 * x + 1/2 * x = x``,
-   STRIP_TAC
-   >> MATCH_MP_TAC (REAL_ARITH ``(2 * (a:real) = 2 * b) ==> (a = b)``)
-   >> RW_TAC std_ss [REAL_ADD_LDISTRIB, REAL_MUL_ASSOC, HALF_CANCEL]
-   >> REAL_ARITH_TAC);
-
-val REAL_SUP_LE_X = store_thm
-  ("REAL_SUP_LE_X",
-   ``!P x. (?r. P r) /\ (!r. P r ==> r <= x) ==> sup P <= x``,
-   RW_TAC real_ss []
-   >> Suff `~(x < sup P)` >- REAL_ARITH_TAC
-   >> STRIP_TAC
-   >> MP_TAC (SPEC ``P:real->bool`` REAL_SUP_LE)
-   >> RW_TAC real_ss [] >|
-   [PROVE_TAC [],
-    PROVE_TAC [],
-    EXISTS_TAC ``x:real``
-    >> RW_TAC real_ss []
-    >> PROVE_TAC [real_lte]]);
-
-val REAL_X_LE_SUP = store_thm
-  ("REAL_X_LE_SUP",
-   ``!P x. (?r. P r) /\ (?z. !r. P r ==> r <= z) /\ (?r. P r /\ x <= r)
-           ==> x <= sup P``,
-   RW_TAC real_ss []
-   >> Suff `!y. P y ==> y <= sup P` >- PROVE_TAC [REAL_LE_TRANS]
-   >> MATCH_MP_TAC REAL_SUP_UBOUND_LE
-   >> PROVE_TAC []);
 
 val REAL_INVINV_ALL = store_thm
   ("REAL_INVINV_ALL",
@@ -230,7 +72,7 @@ val REAL_INVINV_ALL = store_thm
 
 val ABS_BETWEEN_LE = store_thm
   ("ABS_BETWEEN_LE",
-   ``!x y d. 0 <= d /\ x - d <= y /\ y <= x + d = abs (y - x) <= d``,
+   ``!x y d. 0 <= d /\ x - d <= y /\ y <= x + d <=> abs (y - x) <= d``,
    RW_TAC std_ss [abs] >|
    [EQ_TAC >- REAL_ARITH_TAC
     >> STRIP_TAC
@@ -263,21 +105,6 @@ val ABS_BETWEEN_LE = store_thm
      >> Q.PAT_ASSUM `0 <= x - y` MP_TAC
      >> KILL_TAC
      >> REAL_ARITH_TAC]]);
-
-val ONE_MINUS_HALF = store_thm
-  ("ONE_MINUS_HALF",
-   ``1 - 1 / 2 = 1 / 2``,
-   MP_TAC (Q.SPEC `1` X_HALF_HALF)
-   >> RW_TAC real_ss []
-   >> MATCH_MP_TAC (REAL_ARITH ``(x + 1 / 2 = y + 1 / 2) ==> (x = y)``)
-   >> RW_TAC std_ss [REAL_SUB_ADD]);
-
-val HALF_LT_1 = store_thm
-  ("HALF_LT_1",
-   ``1 / 2 < 1``,
-   ONCE_REWRITE_TAC [GSYM REAL_INV_1OVER, GSYM REAL_INV1]
-   >> MATCH_MP_TAC REAL_LT_INV
-   >> RW_TAC arith_ss [REAL_LT]);
 
 val REAL_POW = store_thm
   ("REAL_POW",
@@ -354,32 +181,32 @@ val REAL_INV_NEG = store_thm
 
 val IN_ZREAL = store_thm
   ("IN_ZREAL",
-   ``!x. x IN zreal = (x = 0)``,
+   ``!x. x IN zreal <=> (x = 0)``,
    RW_TAC std_ss [zreal_def, SPECIFICATION]);
 
 val IN_NZREAL = store_thm
   ("IN_NZREAL",
-   ``!x. x IN nzreal = ~(x = 0)``,
+   ``!x. x IN nzreal <=> ~(x = 0)``,
    RW_TAC std_ss [nzreal_def, SPECIFICATION]);
 
 val IN_POSREAL = store_thm
   ("IN_POSREAL",
-   ``!x. x IN posreal = 0 < x``,
+   ``!x. x IN posreal <=> 0 < x``,
    RW_TAC std_ss [posreal_def, SPECIFICATION]);
 
 val IN_NNEGREAL = store_thm
   ("IN_NNEGREAL",
-   ``!x. x IN nnegreal = 0 <= x``,
+   ``!x. x IN nnegreal <=> 0 <= x``,
    RW_TAC std_ss [nnegreal_def, SPECIFICATION]);
 
 val IN_NEGREAL = store_thm
   ("IN_NEGREAL",
-   ``!x. x IN negreal = 0 < ~x``,
+   ``!x. x IN negreal <=> 0 < ~x``,
    RW_TAC std_ss [negreal_def, SPECIFICATION]);
 
 val IN_NPOSREAL = store_thm
   ("IN_NPOSREAL",
-   ``!x. x IN nposreal = 0 <= ~x``,
+   ``!x. x IN nposreal <=> 0 <= ~x``,
    RW_TAC std_ss [nposreal_def, SPECIFICATION]);
 
 val POSREAL_ALT = store_thm
@@ -509,16 +336,16 @@ val REAL_DIV_SUBTYPE = store_thm
 
 val REAL_MULT_EQ_CANCEL = store_thm
   ("REAL_MULT_EQ_CANCEL",
-   ``!x y z : real. ~(x = 0) ==> ((x * y = z) = (y = inv x * z))``,
+   ``!x y z : real. ~(x = 0) ==> ((x * y = z) <=> (y = inv x * z))``,
    Strip
-   >> Suff `(x * y = z) = (x = 0) \/ (y = inv x * z)` >- PROVE_TAC []
+   >> Suff `(x * y = z) <=> (x = 0) \/ (y = inv x * z)` >- PROVE_TAC []
    >> REWRITE_TAC [GSYM REAL_EQ_MUL_LCANCEL]
    >> RW_TAC std_ss [REAL_MUL_ASSOC, REAL_MUL_RINV]
    >> RW_TAC real_ss []);
 
 val REAL_MULT_LE_CANCEL = store_thm
   ("REAL_MULT_LE_CANCEL",
-   ``!x y z : real. 0 < x ==> ((x * y <= z) = (y <= inv x * z))``,
+   ``!x y z : real. 0 < x ==> ((x * y <= z) <=> (y <= inv x * z))``,
    Strip
    >> Suff `(x * y <= z) = (x * y <= x * (inv x * z))`
    >- PROVE_TAC [REAL_LE_LMUL]
@@ -535,177 +362,6 @@ val INV_DIFF_SUC = store_thm
    >> Know `&n + 1 - &n = 1` >- REAL_ARITH_TAC
    >> RW_TAC std_ss [GSYM REAL_INV_1OVER]
    >> RW_TAC std_ss [GSYM REAL, REAL_MUL, GSYM ADD1]);
-
-val SUMS_EQ = store_thm
-  ("SUMS_EQ",
-   ``!f x. f sums x = summable f /\ (suminf f = x)``,
-   PROVE_TAC [SUM_SUMMABLE, SUM_UNIQ, summable]);
-
-val SER_POS = store_thm
-  ("SER_POS",
-   ``!f. summable f /\ (!n. 0 <= f n) ==> 0 <= suminf f``,
-   RW_TAC std_ss []
-   >> MP_TAC (Q.SPECL [`f`, `0`] SER_POS_LE)
-   >> RW_TAC std_ss [sum]);
-
-val SER_POS_MONO = store_thm
-  ("SER_POS_MONO",
-   ``!f. (!n. 0 <= f n) ==> mono (\n. sum (0, n) f)``,
-   RW_TAC std_ss [mono]
-   >> DISJ1_TAC
-   >> HO_MATCH_MP_TAC TRIANGLE_2D_NUM
-   >> Induct >- RW_TAC arith_ss [REAL_LE_REFL]
-   >> RW_TAC std_ss [ADD_CLAUSES]
-   >> MATCH_MP_TAC REAL_LE_TRANS
-   >> Q.EXISTS_TAC `sum (0, d + n) f`
-   >> RW_TAC real_ss [sum]
-   >> Q.PAT_ASSUM `!n. 0 <= f n` (MP_TAC o Q.SPEC `d + n`)
-   >> REAL_ARITH_TAC);
-
-val POS_SUMMABLE = store_thm
-  ("POS_SUMMABLE",
-   ``!f. (!n. 0 <= f n) /\ (?x. !n. sum (0, n) f <= x) ==> summable f``,
-   RW_TAC std_ss [summable, sums, GSYM convergent]
-   >> MATCH_MP_TAC SEQ_BCONV
-   >> RW_TAC std_ss [SER_POS_MONO, netsTheory.MR1_BOUNDED]
-   >> Q.EXISTS_TAC `x + 1`
-   >> Q.EXISTS_TAC `N`
-   >> RW_TAC arith_ss []
-   >> RW_TAC std_ss [abs, SUM_POS]
-   >> Q.PAT_ASSUM `!n. P n` (MP_TAC o Q.SPEC `n`)
-   >> REAL_ARITH_TAC);
-
-val SUMMABLE_LE = store_thm
-  ("SUMMABLE_LE",
-   ``!f x. summable f /\ (!n. sum (0, n) f <= x) ==> suminf f <= x``,
-   Strip
-   >> Suff `0 < suminf f - x ==> F` >- REAL_ARITH_TAC
-   >> Strip
-   >> Know `(\n. sum (0, n) f) --> suminf f`
-   >- RW_TAC std_ss [GSYM sums, SUMMABLE_SUM]
-   >> RW_TAC std_ss [SEQ]
-   >> Q.EXISTS_TAC `suminf f - x`
-   >> RW_TAC std_ss []
-   >> Q.EXISTS_TAC `N`
-   >> Q.PAT_X_ASSUM `!n. P n` (MP_TAC o Q.SPEC `N`)
-   >> RW_TAC real_ss []
-   >> ONCE_REWRITE_TAC [ABS_SUB]
-   >> Know `0 <= suminf f - sum (0, N) f`
-   >- (rpt (POP_ASSUM MP_TAC)
-       >> REAL_ARITH_TAC)
-   >> RW_TAC std_ss [abs]
-   >> rpt (POP_ASSUM MP_TAC)
-   >> REAL_ARITH_TAC);
-
-val LE_INF = store_thm
-  ("LE_INF",
-   ``!p r. (?x. x IN p) /\ (!x. x IN p ==> r <= x) ==> r <= inf p``,
-   RW_TAC std_ss [INF_DEF_ALT, SPECIFICATION]
-   >> POP_ASSUM MP_TAC
-   >> ONCE_REWRITE_TAC [GSYM REAL_NEGNEG]
-   >> Q.SPEC_TAC (`~r`, `r`)
-   >> RW_TAC real_ss [REAL_NEGNEG, REAL_LE_NEG]
-   >> MATCH_MP_TAC REAL_SUP_LE_X
-   >> RW_TAC std_ss []
-   >> PROVE_TAC [REAL_NEGNEG]);
-
-val INF_LE = store_thm
-  ("INF_LE",
-   ``!p r.
-       (?z. !x. x IN p ==> z <= x) /\ (?x. x IN p /\ x <= r) ==> inf p <= r``,
-   RW_TAC std_ss [INF_DEF_ALT, SPECIFICATION]
-   >> POP_ASSUM MP_TAC
-   >> ONCE_REWRITE_TAC [GSYM REAL_NEGNEG]
-   >> Q.SPEC_TAC (`~r`, `r`)
-   >> RW_TAC real_ss [REAL_NEGNEG, REAL_LE_NEG]
-   >> MATCH_MP_TAC REAL_X_LE_SUP
-   >> RW_TAC std_ss []
-   >> PROVE_TAC [REAL_NEGNEG, REAL_LE_NEG]);
-
-val REAL_LE_EPSILON = store_thm
-  ("REAL_LE_EPSILON",
-   ``!x y : real. (!e. 0 < e ==> x <= y + e) ==> x <= y``,
-   RW_TAC std_ss []
-   >> Suff `~(0 < x - y)` >- REAL_ARITH_TAC
-   >> STRIP_TAC
-   >> Q.PAT_X_ASSUM `!e. P e` MP_TAC
-   >> RW_TAC std_ss []
-   >> Know `!a b c : real. ~(a <= b + c) = c < a - b` >- REAL_ARITH_TAC
-   >> DISCH_THEN (ONCE_REWRITE_TAC o wrap)
-   >> PROVE_TAC [REAL_DOWN]);
-
-val SER_POS_COMPARE = store_thm
-  ("SER_POS_COMPARE",
-   ``!f g.
-       (!n. 0 <= f n) /\ summable g /\ (!n. f n <= g n) ==>
-       summable f /\ suminf f <= suminf g``,
-   Reverse (rpt (STRONG_CONJ_TAC ORELSE STRIP_TAC))
-   >- PROVE_TAC [SER_LE]
-   >> MATCH_MP_TAC SER_COMPAR
-   >> Q.EXISTS_TAC `g`
-   >> RW_TAC std_ss []
-   >> Q.EXISTS_TAC `0`
-   >> RW_TAC arith_ss [abs]);
-
-val INF_GREATER = store_thm
-  ("INF_GREATER",
-   ``!p z.
-       (?x. x IN p) /\ inf p < z ==>
-       (?x. x IN p /\ x < z)``,
-   RW_TAC std_ss []
-   >> Suff `~(!x. x IN p ==> ~(x < z))` >- PROVE_TAC []
-   >> REWRITE_TAC [GSYM real_lte]
-   >> STRIP_TAC
-   >> Q.PAT_X_ASSUM `inf p < z` MP_TAC
-   >> RW_TAC std_ss [GSYM real_lte]
-   >> MATCH_MP_TAC LE_INF
-   >> PROVE_TAC []);
-
-val INF_CLOSE = store_thm
-  ("INF_CLOSE",
-   ``!p e.
-       (?x. x IN p) /\ 0 < e ==> (?x. x IN p /\ x < inf p + e)``,
-   RW_TAC std_ss []
-   >> MATCH_MP_TAC INF_GREATER
-   >> CONJ_TAC >- PROVE_TAC []
-   >> POP_ASSUM MP_TAC
-   >> REAL_ARITH_TAC);
-
-val SUMINF_POS = store_thm
-  ("SUMINF_POS",
-   ``!f. (!n. 0 <= f n) /\ summable f ==> 0 <= suminf f``,
-   RW_TAC std_ss []
-   >> Know `0 = sum (0, 0) f` >- RW_TAC std_ss [sum]
-   >> DISCH_THEN (ONCE_REWRITE_TAC o wrap)
-   >> MATCH_MP_TAC SER_POS_LE
-   >> RW_TAC std_ss []);
-
-val POW_HALF_SER = store_thm
-  ("POW_HALF_SER",
-   ``(\n. (1 / 2) pow (n + 1)) sums 1``,
-   Know `(\n. (1 / 2) pow n) sums inv (1 - (1 / 2))`
-   >- (MATCH_MP_TAC GP
-       >> RW_TAC std_ss [abs, HALF_POS, REAL_LT_IMP_LE, HALF_LT_1])
-   >> RW_TAC std_ss [ONE_MINUS_HALF, REAL_INV_INV, GSYM REAL_INV_1OVER,
-                     GSYM ADD1, pow]
-   >> Know `1 = inv 2 * 2`
-   >- RW_TAC arith_ss [REAL_MUL_LINV, REAL_INJ]
-   >> DISCH_THEN (ONCE_REWRITE_TAC o wrap)
-   >> HO_MATCH_MP_TAC SER_CMUL
-   >> RW_TAC std_ss []);
-
-val SUMINF_ADD = store_thm
-  ("SUMINF_ADD",
-   ``!f g.
-       summable f /\ summable g ==>
-       summable (\n. f n + g n) /\
-       (suminf f + suminf g = suminf (\n. f n + g n))``,
-   RW_TAC std_ss [] \\
- ( Know `f sums suminf f /\ g sums suminf g` >- PROVE_TAC [SUMMABLE_SUM]
-   >> STRIP_TAC
-   >> Know `(\n. f n + g n) sums (suminf f + suminf g)`
-   >- RW_TAC std_ss [SER_ADD]
-   >> RW_TAC std_ss [SUMS_EQ] ));
 
 val ABS_TRIANGLE = store_thm
   ("ABS_TRIANGLE",
@@ -747,344 +403,12 @@ val INCREASING_SEQ = store_thm
    >> POP_ASSUM MP_TAC
    >> REAL_ARITH_TAC);
 
-val SUM_PICK = store_thm
-  ("SUM_PICK",
-   ``!n k x. sum (0, n) (\m. if m = k then x else 0) = if k < n then x else 0``,
-   Induct >- RW_TAC arith_ss [sum]
-   >> RW_TAC arith_ss [sum, REAL_ADD_RID, REAL_ADD_LID]
-   >> Suff `F` >- PROVE_TAC []
-   >> NTAC 2 (POP_ASSUM MP_TAC)
-   >> DECIDE_TAC);
-
-val SUM_LT = store_thm
-  ("SUM_LT",
-   ``!f g m n.
-       (!r. m <= r /\ r < n + m ==> f r < g r) /\ 0 < n ==>
-       sum (m,n) f < sum (m,n) g``,
-   RW_TAC std_ss []
-   >> POP_ASSUM MP_TAC
-   >> Cases_on `n` >- RW_TAC arith_ss []
-   >> RW_TAC arith_ss []
-   >> Induct_on `n'` >- RW_TAC arith_ss [sum, REAL_ADD_LID]
-   >> ONCE_REWRITE_TAC [sum]
-   >> Strip
-   >> MATCH_MP_TAC REAL_LT_ADD2
-   >> CONJ_TAC
-   >- (Q.PAT_X_ASSUM `a ==> b` MATCH_MP_TAC
-       >> RW_TAC arith_ss [])
-   >> RW_TAC arith_ss []);
-
 val SUM_CONST = store_thm
   ("SUM_CONST",
    ``!n r. sum (0,n) (K r) = &n * r``,
    Induct >- RW_TAC real_ss [sum]
    >> RW_TAC bool_ss [sum, ADD1, K_THM, GSYM REAL_ADD, REAL_ADD_RDISTRIB]
    >> RW_TAC real_ss []);
-
-val SUMINF_2D = store_thm
-  ("SUMINF_2D",
-   ``!f g h.
-       (!m n. 0 <= f m n) /\ (!n. f n sums g n) /\ summable g /\
-       BIJ h UNIV (UNIV CROSS UNIV) ==>
-       (UNCURRY f o h) sums suminf g``,
-   RW_TAC std_ss []
-   >> RW_TAC std_ss [sums]
-   >> Know `g sums suminf g` >- PROVE_TAC [SUMMABLE_SUM]
-   >> Q.PAT_X_ASSUM `!n. P n` MP_TAC
-   >> RW_TAC std_ss [SUMS_EQ, FORALL_AND_THM]
-   >> MATCH_MP_TAC INCREASING_SEQ
-   >> CONJ_TAC
-   >- (RW_TAC std_ss [sum, o_THM, ADD_CLAUSES]
-       >> Cases_on `h n`
-       >> RW_TAC std_ss [UNCURRY_DEF]
-       >> Q.PAT_X_ASSUM `!m n. 0 <= f m n` (MP_TAC o Q.SPECL [`q`, `r`])
-       >> REAL_ARITH_TAC)
-   >> Know `!m. 0 <= g m`
-   >- (STRIP_TAC
-       >> Suff `0 <= suminf (f m)` >- PROVE_TAC []
-       >> MATCH_MP_TAC SER_POS
-       >> PROVE_TAC [])
-   >> STRIP_TAC
-   >> CONJ_TAC
-   >- (RW_TAC std_ss []
-       >> MP_TAC (Q.SPECL [`h`, `n`] NUM_2D_BIJ_BIG_SQUARE)
-       >> ASM_REWRITE_TAC []
-       >> STRIP_TAC
-       >> MATCH_MP_TAC REAL_LE_TRANS
-       >> Q.EXISTS_TAC `sum (0,k) g`
-       >> Reverse CONJ_TAC
-       >- (MATCH_MP_TAC SER_POS_LE
-           >> PROVE_TAC [])
-       >> MATCH_MP_TAC REAL_LE_TRANS
-       >> Q.EXISTS_TAC `sum (0,k) (\m. sum (0,k) (f m))`
-       >> Reverse CONJ_TAC
-       >- (MATCH_MP_TAC SUM_LE
-           >> RW_TAC std_ss []
-           >> Q.PAT_X_ASSUM `!n. suminf (f n) = g n` (REWRITE_TAC o wrap o GSYM)
-           >> MATCH_MP_TAC SER_POS_LE
-           >> PROVE_TAC [])
-       >> Suff
-          `!j.
-             j <= n ==>
-             (sum (0, j) (UNCURRY f o h) =
-              sum (0, k)
-              (\m. sum (0, k)
-               (\n. if (?i. i < j /\ (h i = (m, n))) then f m n else 0)))`
-       >- (DISCH_THEN (MP_TAC o Q.SPEC `n`)
-           >> REWRITE_TAC [LESS_EQ_REFL]
-           >> DISCH_THEN (ONCE_REWRITE_TAC o wrap)
-           >> MATCH_MP_TAC SUM_LE
-           >> RW_TAC std_ss []
-           >> MATCH_MP_TAC SUM_LE
-           >> RW_TAC std_ss [REAL_LE_REFL])
-       >> Induct >- RW_TAC arith_ss [sum, SUM_0]
-       >> RW_TAC std_ss [sum]
-       >> Q.PAT_X_ASSUM `p ==> q` MP_TAC
-       >> RW_TAC arith_ss []
-       >> Know
-          `!m n.
-             (?i. i < SUC j /\ (h i = (m,n))) =
-             (?i. i < j /\ (h i = (m,n))) \/ (h j = (m, n))`
-       >- (RW_TAC std_ss []
-           >> Suff `!i. i < SUC j = i < j \/ (i = j)`
-           >- PROVE_TAC []
-           >> DECIDE_TAC)
-       >> DISCH_THEN (REWRITE_TAC o wrap)
-       >> Know
-          `!m n.
-             (if (?i. i < j /\ (h i = (m,n))) \/ (h j = (m,n)) then f m n
-              else 0) =
-             (if (?i. i < j /\ (h i = (m,n))) then f m n else 0) +
-             (if (h j = (m,n)) then f m n else 0)`
-       >- (Strip
-           >> Suff `(?i. i < j /\ (h i = (m,n'))) ==> ~(h j = (m,n'))`
-           >- PROVE_TAC [REAL_ADD_LID, REAL_ADD_RID]
-           >> RW_TAC std_ss []
-           >> Q.PAT_X_ASSUM `BIJ a b c` MP_TAC
-           >> RW_TAC std_ss [BIJ_DEF, INJ_DEF, IN_UNIV, IN_CROSS]
-           >> PROVE_TAC [prim_recTheory.LESS_REFL])
-       >> DISCH_THEN (ONCE_REWRITE_TAC o wrap)
-       >> RW_TAC std_ss [SUM_ADD]
-       >> POP_ASSUM K_TAC
-       >> Suff
-          `(UNCURRY f o h) j =
-           sum (0,k)
-           (\m. sum (0,k) (\n. (if h j = (m,n) then f m n else 0)))`
-       >- (KILL_TAC
-           >> Q.SPEC_TAC
-              (`(sum (0,k)
-                 (\m.
-                  sum (0,k)
-                  (\n. if ?i. i < j /\ (h i = (m,n)) then f m n else 0)))`,
-               `r1`)
-           >> Q.SPEC_TAC
-              (`sum (0,k)
-                (\m. sum (0,k) (\n. (if h j = (m,n) then f m n else 0)))`,
-               `r2`)
-           >> RW_TAC std_ss [])
-       >> Cases_on `h j`
-       >> RW_TAC std_ss [o_THM, UNCURRY_DEF]
-       >> Know
-          `!m n.
-             (if (q = m) /\ (r = n) then f m n else 0) =
-             (if (n = r) then if (m = q) then f m n else 0 else 0)`
-       >- PROVE_TAC []
-       >> DISCH_THEN (REWRITE_TAC o wrap)
-       >> Q.PAT_X_ASSUM `a SUBSET b` MP_TAC
-       >> RW_TAC std_ss [SUBSET_DEF, IN_IMAGE, IN_COUNT, IN_CROSS]
-       >> Suff `q < k /\ r < k`
-       >- RW_TAC std_ss [SUM_PICK]
-       >> POP_ASSUM (MP_TAC o Q.SPEC `h (j:num)`)
-       >> Suff `j < n`
-       >- (RW_TAC std_ss []
-           >> PROVE_TAC [])
-       >> DECIDE_TAC)
-   >> RW_TAC std_ss []
-   >> Know `?M. 0 < M /\ suminf g < sum (0, M) g + e / 2`
-   >- (Know `g sums suminf g` >- PROVE_TAC [SUMMABLE_SUM]
-       >> RW_TAC std_ss [sums, SEQ]
-       >> POP_ASSUM (MP_TAC o Q.SPEC `e / 2`)
-       >> RW_TAC std_ss [REAL_LT_HALF1, GREATER_EQ]
-       >> POP_ASSUM (MP_TAC o Q.SPEC `SUC N`)
-       >> ONCE_REWRITE_TAC [ABS_SUB]
-       >> Know `sum (0, SUC N) g <= suminf g`
-       >- (MATCH_MP_TAC SER_POS_LE
-           >> RW_TAC std_ss [])
-       >> Reverse (RW_TAC arith_ss [abs])
-       >- (Suff `F` >- PROVE_TAC []
-           >> POP_ASSUM K_TAC
-           >> POP_ASSUM MP_TAC
-           >> POP_ASSUM MP_TAC
-           >> REAL_ARITH_TAC)
-       >> Q.EXISTS_TAC `SUC N`
-       >> CONJ_TAC >- DECIDE_TAC
-       >> POP_ASSUM MP_TAC
-       >> REAL_ARITH_TAC)
-   >> RW_TAC std_ss []
-   >> Suff `?k. sum (0, M) g < sum (0, k) (UNCURRY f o h) + e / 2`
-   >- (Strip
-       >> Q.EXISTS_TAC `k`
-       >> Know
-          `sum (0, M) g + e / 2 < sum (0, k) (UNCURRY f o h) + (e / 2 + e / 2)`
-       >- (POP_ASSUM MP_TAC
-           >> REAL_ARITH_TAC)
-       >> POP_ASSUM K_TAC
-       >> POP_ASSUM MP_TAC
-       >> REWRITE_TAC [REAL_HALF_DOUBLE]
-       >> REAL_ARITH_TAC)
-   >> POP_ASSUM K_TAC
-   >> Know `!m. ?N. g m < sum (0, N) (f m) + (e / 2) / & M`
-   >- (Know `!m. f m sums g m`
-       >- RW_TAC std_ss [SUMS_EQ]
-       >> RW_TAC std_ss [sums, SEQ]
-       >> POP_ASSUM (MP_TAC o Q.SPECL [`m`, `(e / 2) / & M`])
-       >> Know `0 < (e / 2) / & M`
-       >- RW_TAC arith_ss [REAL_LT_DIV, REAL_NZ_IMP_LT]
-       >> DISCH_THEN (REWRITE_TAC o wrap)
-       >> RW_TAC std_ss [GREATER_EQ]
-       >> POP_ASSUM (MP_TAC o Q.SPEC `N`)
-       >> ONCE_REWRITE_TAC [ABS_SUB]
-       >> Know `sum (0, N) (f m) <= g m`
-       >- (Q.PAT_X_ASSUM `!n. P n = Q n` (REWRITE_TAC o wrap o GSYM)
-           >> MATCH_MP_TAC SER_POS_LE
-           >> RW_TAC std_ss [])
-       >> Reverse (RW_TAC arith_ss [abs])
-       >- (POP_ASSUM K_TAC
-           >> Suff `F` >- PROVE_TAC []
-           >> NTAC 2 (POP_ASSUM MP_TAC)
-           >> REAL_ARITH_TAC)
-       >> Q.EXISTS_TAC `N`
-       >> POP_ASSUM MP_TAC
-       >> REAL_ARITH_TAC)
-   >> DISCH_THEN (MP_TAC o CONV_RULE SKOLEM_CONV)
-   >> RW_TAC std_ss []
-   >> Know `?c. M <= c /\ !m. m < M ==> N m <= c`
-   >- (KILL_TAC
-       >> Induct_on `M` >- RW_TAC arith_ss []
-       >> Strip
-       >> Q.EXISTS_TAC `MAX (SUC c) (N M)`
-       >> RW_TAC arith_ss [X_LE_MAX, LT_SUC]
-       >> PROVE_TAC [LESS_EQ_REFL, LE])
-   >> Strip
-   >> MP_TAC (Q.SPECL [`h`, `c`] NUM_2D_BIJ_SMALL_SQUARE)
-   >> ASM_REWRITE_TAC []
-   >> DISCH_THEN (Q.X_CHOOSE_TAC `k`)
-   >> Q.EXISTS_TAC `k`
-   >> MATCH_MP_TAC REAL_LTE_TRANS
-   >> Q.EXISTS_TAC `sum (0, M) (\m. sum (0, N m) (f m) + e / 2 / &M)`
-   >> CONJ_TAC
-   >- (MATCH_MP_TAC SUM_LT
-       >> RW_TAC arith_ss [])
-   >> RW_TAC std_ss [SUM_ADD, GSYM K_PARTIAL, SUM_CONST]
-   >> Know `!x. & M * (x / & M) = x`
-   >- (RW_TAC std_ss [real_div]
-       >> Suff `(& M * inv (& M)) * x = x`
-       >- PROVE_TAC [REAL_MUL_ASSOC, REAL_MUL_SYM]
-       >> Suff `~(& M = 0)` >- RW_TAC std_ss [REAL_MUL_RINV, REAL_MUL_LID]
-       >> RW_TAC arith_ss [REAL_INJ])
-   >> DISCH_THEN (REWRITE_TAC o wrap)
-   >> RW_TAC std_ss [REAL_LE_RADD]
-   >> Suff
-      `sum (0,M) (\m. sum (0,N m) (f m)) =
-       sum (0, k)
-       (\k.
-          if ?m n. m < M /\ n < N m /\ (h k = (m, n)) then (UNCURRY f o h) k
-          else 0)`
-   >- (RW_TAC std_ss []
-       >> MATCH_MP_TAC SUM_LE
-       >> RW_TAC std_ss [o_THM, REAL_LE_REFL]
-       >> Cases_on `h r`
-       >> RW_TAC std_ss [UNCURRY_DEF])
-   >> NTAC 3 (POP_ASSUM MP_TAC)
-   >> Q.PAT_X_ASSUM `BIJ h a b` MP_TAC
-   >> KILL_TAC
-   >> RW_TAC std_ss []
-   >> Induct_on `M` >- RW_TAC arith_ss [sum, SUM_ZERO]
-   >> RW_TAC arith_ss [sum, LT_SUC]
-   >> Q.PAT_X_ASSUM `a ==> b` K_TAC
-   >> Know
-      `!k'.
-         (?m n. (m < M \/ (m = M)) /\ n < N m /\ (h k' = (m, n))) =
-         (?m n. m < M /\ n < N m /\ (h k' = (m, n))) \/
-         (?n. n < N M /\ (h k' = (M, n)))`
-   >- PROVE_TAC []
-   >> DISCH_THEN (REWRITE_TAC o wrap)
-   >> Know
-      `!k'.
-         (if (?m n. m < M /\ n < N m /\ (h k' = (m,n))) \/
-             (?n. n < N M /\ (h k' = (M,n)))
-          then UNCURRY f (h k')
-          else 0) =
-         (if (?m n. m < M /\ n < N m /\ (h k' = (m,n))) then UNCURRY f (h k')
-          else 0) +
-         (if (?n. n < N M /\ (h k' = (M,n))) then UNCURRY f (h k')
-          else 0)`
-   >- (STRIP_TAC
-       >> Suff
-          `(?m n. m < M /\ n < N m /\ (h k' = (m,n))) ==>
-           ~(?n. n < N M /\ (h k' = (M,n)))`
-       >- PROVE_TAC [REAL_ADD_RID, REAL_ADD_LID]
-       >> Cases_on `h k'`
-       >> RW_TAC arith_ss [])
-   >> DISCH_THEN (REWRITE_TAC o wrap)
-   >> RW_TAC std_ss [SUM_ADD, REAL_EQ_LADD]
-   >> Know `N M <= c` >- PROVE_TAC []
-   >> POP_ASSUM K_TAC
-   >> Q.SPEC_TAC (`N M`, `l`)
-   >> Induct >- RW_TAC real_ss [sum, SUM_0]
-   >> RW_TAC arith_ss [sum, LT_SUC]
-   >> Q.PAT_X_ASSUM `a ==> b` K_TAC
-   >> Know
-      `!k'.
-         (?n. (n < l \/ (n = l)) /\ (h k' = (M,n))) =
-         (?n. n < l /\ (h k' = (M,n))) \/ (h k' = (M, l))`
-   >- PROVE_TAC []
-   >> DISCH_THEN (REWRITE_TAC o wrap)
-   >> Know
-      `!k'.
-         (if (?n. n < l /\ (h k' = (M,n))) \/ (h k' = (M, l)) then
-            UNCURRY f (h k')
-          else 0) =
-         (if (?n. n < l /\ (h k' = (M,n))) then UNCURRY f (h k') else 0) +
-         (if (h k' = (M, l)) then UNCURRY f (h k') else 0)`
-   >- (STRIP_TAC
-       >> Suff `(?n. n < l /\ (h k' = (M,n))) ==> ~(h k' = (M, l))`
-       >- PROVE_TAC [REAL_ADD_LID, REAL_ADD_RID]
-       >> Cases_on `h k'`
-       >> RW_TAC arith_ss [])
-   >> DISCH_THEN (REWRITE_TAC o wrap)
-   >> RW_TAC std_ss [SUM_ADD, REAL_EQ_LADD]
-   >> Q.PAT_X_ASSUM `a SUBSET b` MP_TAC
-   >> RW_TAC std_ss [SUBSET_DEF, IN_CROSS, IN_COUNT, IN_IMAGE]
-   >> POP_ASSUM (MP_TAC o Q.SPEC `(M, l)`)
-   >> RW_TAC arith_ss []
-   >> Suff `!k'. (h k' = (M, l)) = (k' = x')`
-   >- (RW_TAC std_ss [SUM_PICK, o_THM]
-       >> Q.PAT_X_ASSUM `(M,l) = a` (REWRITE_TAC o wrap o GSYM)
-       >> RW_TAC std_ss [UNCURRY_DEF])
-   >> Q.PAT_X_ASSUM `BIJ h a b` MP_TAC
-   >> RW_TAC std_ss [BIJ_DEF, INJ_DEF, IN_UNIV, IN_CROSS]
-   >> PROVE_TAC []);
-
-val REAL_INV_INJ = store_thm
-  ("REAL_INV_INJ",
-   ``!x y. (inv x = inv y) = (x = y)``,
-   RW_TAC std_ss []
-   >> Reverse EQ_TAC >- RW_TAC std_ss []
-   >> RW_TAC std_ss []
-   >> ONCE_REWRITE_TAC [GSYM REAL_INV_INV]
-   >> RW_TAC std_ss []);
-
-val POW_HALF_SMALL = store_thm
-  ("POW_HALF_SMALL",
-   ``!e. 0 < e ==> ?n. (1 / 2) pow n < e``,
-   RW_TAC std_ss []
-   >> MP_TAC (Q.SPEC `1 / 2` SEQ_POWER)
-   >> RW_TAC std_ss [abs, HALF_LT_1, HALF_POS, REAL_LT_IMP_LE, SEQ]
-   >> POP_ASSUM (MP_TAC o Q.SPEC `e`)
-   >> RW_TAC std_ss [REAL_SUB_RZERO, POW_HALF_POS, REAL_LT_IMP_LE,
-                      GREATER_EQ]
-   >> PROVE_TAC [LESS_EQ_REFL]);
 
 val LOG2_SUC = store_thm
   ("LOG2_SUC",
@@ -1115,20 +439,6 @@ val LOG2_SUC = store_thm
    >> MATCH_MP_TAC EXP2_MONO_LE
    >> MP_TAC (Q.SPEC `n + 1` LOG2_LOWER)
    >> RW_TAC arith_ss []);
-
-val LE_SEQ_IMP_LE_LIM = store_thm
-  ("LE_SEQ_IMP_LE_LIM",
-   ``!x y f. (!n. x <= f n) /\ f --> y ==> x <= y``,
-   RW_TAC std_ss [SEQ]
-   >> MATCH_MP_TAC REAL_LE_EPSILON
-   >> RW_TAC std_ss []
-   >> Q.PAT_X_ASSUM `!e. P e` (MP_TAC o Q.SPEC `e`)
-   >> RW_TAC std_ss []
-   >> POP_ASSUM (MP_TAC o Q.SPEC `N`)
-   >> Q.PAT_X_ASSUM `!n. P n` (MP_TAC o Q.SPEC `N`)
-   >> RW_TAC arith_ss [abs]
-   >> REPEAT (POP_ASSUM MP_TAC)
-   >> REAL_ARITH_TAC);
 
 val SER_POS_COMPAR = store_thm
   ("SER_POS_COMPAR",
@@ -1228,7 +538,7 @@ val SER_BIJ_COMPRESS1 = store_thm
            >> Q.EXISTS_TAC `SUC (MAX N (h n))`
            >> STRIP_TAC
            >> DISCH_THEN (MP_TAC o REWRITE_RULE [LT_SUC])
-           >> Know `!a b. a < SUC b = a <= b`
+           >> Know `!a b. a < SUC b <=> a <= b`
            >- (Cases >> STRIP_TAC >> KILL_TAC >> DECIDE_TAC)
            >> RW_TAC std_ss [X_LE_MAX]
            >> PROVE_TAC [LESS_IMP_LESS_OR_EQ, LESS_EQ_REFL])
@@ -1237,7 +547,7 @@ val SER_BIJ_COMPRESS1 = store_thm
        >> STRIP_TAC
        >> MATCH_MP_TAC REAL_LE_TRANS
        >> Q.EXISTS_TAC `sum (0, N n) f`
-       >> REVERSE CONJ_TAC
+       >> Reverse CONJ_TAC
        >- (MATCH_MP_TAC SER_POS_LE
            >> RW_TAC std_ss [])
        >> Know `sum (0, N n) f = sum (0, N n) (f o I)`
@@ -1296,7 +606,7 @@ val SER_BIJ_COMPRESS1 = store_thm
        ((\x. sum_CASE x f (K 0)) o
         (\i. if i < n then INL (h i) else INR (i - n)))`
    >- (KILL_TAC
-       >> REVERSE (Induct_on `N`)
+       >> Reverse (Induct_on `N`)
        >- RW_TAC arith_ss [sum, o_THM, ADD_CLAUSES, K_THM, REAL_ADD_RID]
        >> RW_TAC arith_ss []
        >> MATCH_MP_TAC SUM_EQ
@@ -1342,7 +652,7 @@ val SER_BIJ_COMPRESS2 = store_thm
        >> RW_TAC std_ss [INTER_SUBSET, IN_INTER]
        >> MATCH_MP_TAC REAL_LE_TRANS
        >> Q.EXISTS_TAC `sum (0, N) (f o h)`
-       >> REVERSE CONJ_TAC
+       >> Reverse CONJ_TAC
        >- (MATCH_MP_TAC SER_POS_LE
            >> RW_TAC std_ss [o_THM])
        >> Know
@@ -1358,7 +668,7 @@ val SER_BIJ_COMPRESS2 = store_thm
         ((\x. sum_CASE x f (K 0)) o
          (\i. if i < N then INL (h i) else INR (i - N)))`
        >- (KILL_TAC
-           >> REVERSE (Induct_on `n`)
+           >> Reverse (Induct_on `n`)
            >- RW_TAC arith_ss [sum, o_THM, ADD_CLAUSES, K_THM, REAL_ADD_RID]
            >> RW_TAC arith_ss []
            >> MATCH_MP_TAC SUM_EQ
@@ -1397,7 +707,7 @@ val SER_BIJ_COMPRESS2 = store_thm
        >> Q.EXISTS_TAC `SUC (MAX N' (h n))`
        >> STRIP_TAC
        >> DISCH_THEN (MP_TAC o REWRITE_RULE [LT_SUC])
-       >> Know `!a b. a < SUC b = a <= b`
+       >> Know `!a b. a < SUC b <=> a <= b`
        >- (Cases >> STRIP_TAC >> KILL_TAC >> DECIDE_TAC)
        >> RW_TAC std_ss [X_LE_MAX]
        >> PROVE_TAC [LESS_IMP_LESS_OR_EQ, LESS_EQ_REFL])
@@ -1434,7 +744,7 @@ val SER_BIJ_COMPRESS = store_thm
   ("SER_BIJ_COMPRESS",
    ``!f h s l.
        (!n. 0 <= f n) /\ BIJ h UNIV s /\ (!n. ~(n IN s) ==> (f n = 0)) ==>
-       ((f o h) sums l = f sums l)``,
+       ((f o h) sums l <=> f sums l)``,
    RW_TAC std_ss [SUMS_EQ]
    >> EQ_TAC >|
    [STRIP_TAC
@@ -1450,7 +760,7 @@ val SER_BIJ = store_thm
   ("SER_BIJ",
    ``!f g h l.
        (!n. 0 <= f n) /\ BIJ h UNIV UNIV ==>
-       ((f o h) sums l = f sums l)``,
+       ((f o h) sums l <=> f sums l)``,
    RW_TAC std_ss []
    >> MATCH_MP_TAC SER_BIJ_COMPRESS
    >> Q.EXISTS_TAC `UNIV`
@@ -1460,16 +770,6 @@ val SUMS_ZERO = store_thm
   ("SUMS_ZERO",
    ``(K 0) sums 0``,
    RW_TAC real_ss [sums, SEQ, SUM_CONST, abs, REAL_SUB_REFL, REAL_LE_REFL]);
-
-val REAL_MUL_IDEMPOT = store_thm
-  ("REAL_MUL_IDEMPOT",
-   ``!r : real. (r * r = r) = (r = 0) \/ (r = 1)``,
-   GEN_TAC
-   >> Reverse EQ_TAC
-   >- (RW_TAC real_ss [] >> RW_TAC std_ss [REAL_MUL_LZERO, REAL_MUL_LID])
-   >> RW_TAC std_ss []
-   >> Know `r * r = 1 * r` >- RW_TAC real_ss []
-   >> RW_TAC std_ss [REAL_EQ_RMUL]);
 
 val GP_REC = store_thm
   ("GP_REC",
@@ -1507,11 +807,6 @@ val REAL_DIV_EQ = store_thm
    >> Know `inv d * b = b * inv d` >- PROVE_TAC [REAL_MUL_SYM]
    >> Rewr
    >> RW_TAC std_ss [GSYM REAL_MUL_ASSOC, REAL_MUL_LINV, REAL_MUL_RID]);
-
-val REAL_DIV_ADD = store_thm
-  ("REAL_DIV_ADD",
-   ``!x y z : real. x / z + y / z = (x + y) / z``,
-   RW_TAC std_ss [real_div, GSYM REAL_ADD_RDISTRIB]);
 
 val REAL_DIV_MUL = store_thm
   ("REAL_DIV_MUL",
@@ -1565,25 +860,6 @@ val ABS_EQ = store_thm
    >> RW_TAC std_ss [SEQ_CONST]
    >> RW_TAC std_ss [SEQ]);
 
-val SEQ_SANDWICH = store_thm
-  ("SEQ_SANDWICH",
-   ``!f g h l.
-       f --> l /\ h --> l /\ (!n. f n <= g n /\ g n <= h n) ==> g --> l``,
-   RW_TAC std_ss [SEQ, GREATER_EQ]
-   >> Q.PAT_X_ASSUM `!e. P e ==> Q e` (MP_TAC o Q.SPEC `e`)
-   >> Q.PAT_X_ASSUM `!e. P e ==> Q e` (MP_TAC o Q.SPEC `e`)
-   >> RW_TAC std_ss []
-   >> Q.EXISTS_TAC `MAX N N'`
-   >> RW_TAC std_ss [MAX_LE_X]
-   >> Q.PAT_X_ASSUM `!e. P e ==> Q e` (MP_TAC o Q.SPEC `n`)
-   >> Q.PAT_X_ASSUM `!e. P e ==> Q e` (MP_TAC o Q.SPEC `n`)
-   >> RW_TAC std_ss []
-   >> REPEAT (POP_ASSUM MP_TAC)
-   >> DISCH_THEN (MP_TAC o Q.SPEC `n`)
-   >> RW_TAC std_ss [abs]
-   >> REPEAT (POP_ASSUM MP_TAC)
-   >> REAL_ARITH_TAC);
-
 val POW_LE_1 = store_thm
   ("POW_LE_1",
    ``!p n. 0 < p /\ p <= 1 ==> p pow n <= 1``,
@@ -1612,8 +888,7 @@ val POW_LE_1_MONO = store_thm
 
 val REAL_LE_MUL_EPSILON = store_thm
   ("REAL_LE_MUL_EPSILON",
-   ``!x y. (!z. 0 < z /\ z < 1 ==> z * x <= y) ==>
-                x <= y``,
+   ``!x y. (!z. 0 < z /\ z < 1 ==> z * x <= y) ==> x <= y``,
     REPEAT STRIP_TAC
     >> Cases_on `x = 0`
     >- (Q.PAT_X_ASSUM `!z. P z` (MP_TAC o Q.SPEC `1/2`) >> RW_TAC real_ss [REAL_HALF_BETWEEN])
@@ -1642,125 +917,18 @@ val REAL_LE_MUL_EPSILON = store_thm
     >> METIS_TAC [REAL_NEG_GT0, REAL_LT_TOTAL, REAL_LE_REFL, REAL_HALF_BETWEEN, REAL_LE_RMUL]);
 
 (* ------------------------------------------------------------------------- *)
-(* ----- Defining real-valued power, log, and log base 2 functions --------- *)
-(* ------------------------------------------------------------------------- *)
-
-val _ = set_fixity "powr" (Infixr 700);
-
-val powr_def = Define
-        `x powr a = exp (a * ln x)`;
-
-val logr_def = Define
-        `logr a x = ln x / ln a`;
-
-val lg_def = Define
-        `lg x = logr 2 x`;
-
-
-val lg_1 = store_thm
-  ("lg_1",
-   ``lg 1 = 0``,
-   RW_TAC real_ss [lg_def, logr_def, LN_1]);
-
-
-val logr_1 = store_thm
-  ("logr_1",
-   ``!b. logr b 1 = 0``,
-   RW_TAC real_ss [logr_def, LN_1]);
-
-
-val lg_nonzero = store_thm
-  ("lg_nonzero",
-   ``!x. (~(x = 0)) /\ (0 <= x) ==>
-                ((~(lg x = 0)) = (~(x = 1)))``,
-   RW_TAC std_ss [REAL_ARITH ``(~(x = 0)) /\ (0 <= x) = 0 < x``]
-   >> RW_TAC std_ss [GSYM lg_1]
-   >> RW_TAC std_ss [lg_def, logr_def, real_div, REAL_EQ_RMUL, REAL_INV_EQ_0]
-   >> (MP_TAC o Q.SPECL [`2`, `1`]) LN_INJ >> RW_TAC real_ss [LN_1]
-   >> RW_TAC std_ss [GSYM LN_1]
-   >> MATCH_MP_TAC LN_INJ
-   >> RW_TAC real_ss []);
-
-val lg_mul = store_thm
-  ("lg_mul",
-   ``!x y. 0 < x /\ 0 < y ==> (lg (x * y) = lg x + lg y)``,
-   RW_TAC real_ss [lg_def, logr_def, LN_MUL]);
-
-val logr_mul = store_thm
-  ("logr_mul",
-   ``!b x y. 0 < x /\ 0 < y ==> (logr b (x * y) = logr b x + logr b y)``,
-   RW_TAC real_ss [logr_def, LN_MUL]);
-
-val lg_2 = store_thm
-  ("lg_2",
-   ``lg 2 = 1``,
-   RW_TAC real_ss [lg_def, logr_def]
-   >> MATCH_MP_TAC REAL_DIV_REFL
-   >> (ASSUME_TAC o Q.SPECL [`1`, `2`]) LN_MONO_LT
-   >> FULL_SIMP_TAC real_ss [LN_1]
-   >> ONCE_REWRITE_TAC [EQ_SYM_EQ]
-   >> MATCH_MP_TAC REAL_LT_IMP_NE
-   >> ASM_REWRITE_TAC []);
-
-val lg_inv = store_thm
-  ("lg_inv",
-   ``!x. 0 < x ==> (lg (inv x) = ~ lg x)``,
-   RW_TAC real_ss [lg_def, logr_def, LN_INV, real_div]);
-
-
-val logr_inv = store_thm
-  ("logr_inv",
-   ``!b x. 0 < x ==> (logr b (inv x) = ~ logr b x)``,
-   RW_TAC real_ss [logr_def, LN_INV, real_div]);
-
-
-val logr_div = store_thm
-  ("logr_div",
-   ``!b x y. 0 < x /\ 0 < y ==>
-        (logr b (x/y) = logr b x - logr b y)``,
-   RW_TAC real_ss [real_div, logr_mul, logr_inv, GSYM real_sub]);
-
-
-val neg_lg = store_thm
-  ("neg_lg",
-  ``!x. 0 < x ==> ((~(lg x)) = lg (inv x))``,
-   RW_TAC real_ss [lg_def, logr_def, real_div]
-   >> `~(ln x * inv (ln 2)) = (~ ln x) * inv (ln 2)` by REAL_ARITH_TAC
-   >> POP_ASSUM (fn thm => ONCE_REWRITE_TAC [thm])
-   >> RW_TAC real_ss [REAL_EQ_RMUL]
-   >> DISJ2_TAC >> ONCE_REWRITE_TAC [EQ_SYM_EQ] >> MATCH_MP_TAC LN_INV
-   >> RW_TAC std_ss []);
-
-val neg_logr = store_thm
-  ("neg_logr",
-  ``!b x. 0 < x ==> ((~(logr b x)) = logr b (inv x))``,
-   RW_TAC real_ss [logr_def, real_div]
-   >> `~(ln x * inv (ln b)) = (~ ln x) * inv (ln b)` by REAL_ARITH_TAC
-   >> POP_ASSUM (fn thm => ONCE_REWRITE_TAC [thm])
-   >> RW_TAC real_ss [REAL_EQ_RMUL]
-   >> DISJ2_TAC >> ONCE_REWRITE_TAC [EQ_SYM_EQ] >> MATCH_MP_TAC LN_INV
-   >> RW_TAC std_ss []);
-
-
-val lg_pow = store_thm
-  ("lg_pow",
-   ``!n. lg (2 pow n) = &n``,
-   RW_TAC real_ss [lg_def, logr_def, LN_POW]
-   >> `~(ln 2 = 0)`
-        by (ONCE_REWRITE_TAC [EQ_SYM_EQ] >> MATCH_MP_TAC REAL_LT_IMP_NE
-            >> MATCH_MP_TAC REAL_LET_TRANS >> Q.EXISTS_TAC `ln 1` >> RW_TAC real_ss [LN_POS, LN_MONO_LT])
-   >> RW_TAC real_ss [real_div, GSYM REAL_MUL_ASSOC, REAL_MUL_RINV]);
-
-
-(* ------------------------------------------------------------------------- *)
 (* --------------------- exp is a convex function -------------------------- *)
 (* ------------------------------------------------------------------------- *)
 
-val convex_fn = Define
-        `convex_fn = {f | !x y t. (0 <= t /\ t <= 1) ==> f (t * x + (1 - t) * y) <= t * f x + (1 - t) * f y}`;
+Definition convex_fn :
+    convex_fn =
+      {f | !x y t. (0 <= t /\ t <= 1) ==>
+                   f (t * x + (1 - t) * y) <= t * f x + (1 - t) * f y}
+End
 
-val concave_fn = Define
-        `concave_fn = {f | (\x. ~ (f x)) IN convex_fn}`;
+Definition concave_fn :
+    concave_fn = {f | (\x. ~ (f x)) IN convex_fn}
+End
 
 val exp_convex_lemma1 = store_thm
   ("exp_convex_lemma1",
@@ -1770,7 +938,8 @@ val exp_convex_lemma1 = store_thm
 
 val exp_convex_lemma2 = store_thm
   ("exp_convex_lemma2",
-   ``!t x. ((\x. (1 - t) * exp x - exp ((1 - t) * x)) diffl (\x. (1-t) * exp x - (1 - t)*exp ((1-t)*x)) x) x``,
+   ``!t x. ((\x. (1 - t) * exp x - exp ((1 - t) * x)) diffl
+            (\x. (1-t) * exp x - (1 - t)*exp ((1-t)*x)) x) x``,
    RW_TAC std_ss []
    >> `(\x. (1 - t) * exp x - exp ((1 - t) * x)) =
        (\x. (\x. (1 - t) * exp x) x - (\x. exp ((1 - t) * x)) x)`
@@ -1894,12 +1063,14 @@ val exp_convex = store_thm
 (* ------------ ln and lg are concave on (0,infty] ------------------------- *)
 (* ------------------------------------------------------------------------- *)
 
-val pos_convex_fn = Define
-        `pos_convex_fn = {f | !x y t. (0 < x /\ 0 < y /\ 0 <= t /\ t <= 1) ==>
-                                f (t * x + (1 - t) * y) <= t * f x + (1 - t) * f y}`;
+Definition pos_convex_fn :
+    pos_convex_fn = {f | !x y t. (0 < x /\ 0 < y /\ 0 <= t /\ t <= 1) ==>
+                                 f (t * x + (1 - t) * y) <= t * f x + (1 - t) * f y}
+End
 
-val pos_concave_fn = Define
-        `pos_concave_fn = {f | (\x. ~ (f x)) IN pos_convex_fn}`;
+Definition pos_concave_fn :
+    pos_concave_fn = {f | (\x. ~ (f x)) IN pos_convex_fn}
+End
 
 val pos_concave_ln = store_thm
   ("pos_concave_ln",
@@ -1941,7 +1112,6 @@ val pos_concave_lg = store_thm
    >> CONJ_TAC >- (RW_TAC real_ss [REAL_LE_INV_EQ] >> MATCH_MP_TAC LN_POS >> RW_TAC real_ss [])
    >> MP_TAC pos_concave_ln
    >> RW_TAC std_ss [pos_concave_fn, pos_convex_fn, EXTENSION, MEM, NOT_IN_EMPTY, GSPECIFICATION]);
-
 
 val pos_concave_logr = store_thm
   ("pos_concave_logr",
